Partial merge of PKI callbacks (missing the OpenSSL PKI provider)

libs/ffi/FFICallbacks.ml
@@ -1,6 +1,12 @@
 type callbacks = int64
 
 external ocaml_ticket_cb: callbacks -> callbacks -> string -> string -> string -> unit = "ocaml_ticket_cb"
+
+external ocaml_cert_select_cb: callbacks -> callbacks -> string -> string -> (callbacks * int) option = "ocaml_cert_select_cb"
+external ocaml_cert_format_cb: callbacks -> callbacks -> callbacks -> string = "ocaml_cert_format_cb"
+external ocaml_cert_sign_cb: callbacks -> callbacks -> callbacks -> int -> string -> string option = "ocaml_cert_sign_cb"
+external ocaml_cert_verify_cb: callbacks -> callbacks -> string -> int -> string*string -> bool = "ocaml_cert_verify_cb"
+
 external _ocaml_send_tcp: callbacks -> string -> int = "ocaml_send_tcp"
 external _ocaml_recv_tcp: callbacks -> string -> int = "ocaml_recv_tcp"
 
