src/tls/TLS.fst
@@ -565,8 +565,7 @@ let sendHandshake_post (#c:connection) (#i:id) (wopt:option (cwriter i c))
 		       then frags1==snoc frags0' (Content.CT_CCS #i (point 1))
 		       else frags1==frags0')))))
 
-#reset-options "--z3rlimit 100 --initial_fuel 0 --max_fuel 0 --initial_ifuel 1 --max_ifuel 1"
-//#set-options "--using_facts_from FStar --using_facts_from Prims --using_facts_from Range --using_facts_from Parse --using_facts_from Connection --using_facts_from Handshake --using_facts_from TLS --using_facts_from TLSError --using_facts_from TLSConstants"
+#reset-options "--z3rlimit 100 --initial_fuel 0 --max_fuel 0 --initial_ifuel 1 --max_ifuel 1 --using_facts_from FStar --using_facts_from Prims --using_facts_from Range --using_facts_from Parse --using_facts_from Connection --using_facts_from Handshake --using_facts_from TLS --using_facts_from TLSError --using_facts_from TLSConstants"
 
 private let sendHandshake
   (#c:connection)
